# Gradient Vanishingê³¼ LSTM

$$\begin{aligned}
o_t&=o(x_t, h_{t-1};W_o) \\
g_t&=g(x_t, h_{t-1};W_g) \\
f_t&=f(x_t, h_{t-1};W_f) \\
i_t&=i(x_t, h_{t-1};W_i) \\
c_t&=f_t\otimes{c_{t-1}}+i_t\otimes{g_t} \\
&=f(x_t, h_{t-1};W_f)\otimes{c_{t-1}}+i(x_t, h_{t-1};W_i)\otimes{g(x_t, h_{t-1};W_g)} \\
h_t&=o_t\otimes\text{tanh}(c_t) \\
\end{aligned}$$

<!--
$$
\frac{\partial{h_t}}{\partial{W_f}}=\frac{\partial{o_t}}{\partial{W_f}}\otimes\text{tanh}(c_t)+o_t\otimes\frac{\partial{\text{tanh}(c_t)}}{\partial{W_f}} \\
\\
\frac{\partial{\text{tanh}(c_t)}}{\partial{W_f}}=\frac{\partial{\text{tanh}(c_t)}}{\partial{c_t}}\frac{\partial{c_t}}{\partial{W_f}} \\
\begin{aligned}
\frac{\partial{c_t}}{\partial{W_f}}&=\frac{\partial{f_t}}{\partial{W_f}}\otimes{c_{t-1}}
    +f_t\otimes\frac{\partial{c_{t-1}}}{\partial{W_f}}
    +\frac{\partial{i_t}}{\partial{W_f}}\otimes{g_t}
    +i_t\otimes\frac{\partial{g_t}}{\partial{W_f}} \\
&={f_t}\otimes\frac{\partial{c_{t-1}}}{\partial{W_f}}+C_t \\
&=f_t\otimes(f_{t-1}\otimes\frac{\partial{c_{t-2}}}{\partial{W_f}}+C_{t-1})+C_t \\
&=f_t\otimes{f_{t-1}}\otimes(f_{t-2}\otimes\frac{\partial{c_{t-3}}}{\partial{W_f}}+C_{t-2})+f_t\otimes{C_{t-1}}+C_t \\
&=\prod_{i=2}^{t}{f_i}\otimes\frac{\partial{c_1}}{\partial{W_f}}+\sum_{i=1}^{t}{C_i\otimes\Big(\prod_{j=i+1}^{t}{f_j}\Big)}
\end{aligned} \\
$$
-->

$$\begin{gathered}
\begin{aligned}
\frac{\partial{c_t}}{\partial{W_f}}&=\frac{\partial{c_t}}{\partial{W_f}}+\frac{\partial{c_t}}{\partial{c_{t-1}}}\frac{\partial{c_{t-1}}}{\partial{W_f}}+\cdots+\frac{\partial{c_t}}{\partial{c_{t-1}}}\frac{\partial{c_{t-1}}}{\partial{c_{t-2}}}\cdots\frac{\partial{c_1}}{\partial{W_f}} \\
&=\frac{\partial{c_t}}{\partial{W_f}}+\frac{\partial{c_{t-1}}}{\partial{W_f}}\frac{\partial{c_t}}{\partial{c_{t-1}}}+\cdots+\frac{\partial{c_1}}{\partial{W_f}}\prod_{i=1}^{t-1}{
    \frac{\partial{c_{i+1}}}{\partial{c_i}}
} \\
&=\sum_{i=1}^{t}{\frac{\partial{c_i}}{\partial{W_f}}\prod_{j=i}^{t-1}{
    \frac{\partial{c_{j+1}}}{\partial{c_j}}}
}
\end{aligned} \\
\\
\\
\begin{aligned}
\frac{\partial{c_t}}{\partial{c_{t-1}}}&=\frac{\partial{f_t}}{\partial{c_{t-1}}}\otimes{c_{t-1}}+f_t\otimes\frac{\partial{c_{t-1}}}{\partial{c_{t-1}}}+\frac{\partial{i_t}}{\partial{c_{t-1}}}\otimes{g_t}+i_t\otimes\frac{\partial{g_t}}{\partial{c_{t-1}}} \\
&=\frac{\partial{f_t}}{\partial{c_{t-1}}}\otimes{c_{t-1}}+f_t+\frac{\partial{i_t}}{\partial{c_{t-1}}}\otimes{g_t}+i_t\otimes\frac{\partial{g_t}}{\partial{c_{t-1}}} \\
&=\frac{\partial{f_t}}{\partial{h_{t-1}}}\frac{\partial{h_{t-1}}}{\partial{c_{t-1}}}\otimes{c_{t-1}}+f_t+\frac{\partial{i_t}}{\partial{h_{t-1}}}\frac{\partial{h_{t-1}}}{\partial{c_{t-1}}}\otimes{g_t}+i_t\otimes\frac{\partial{g_t}}{\partial{h_{t-1}}}\frac{\partial{h_{t-1}}}{\partial{c_{t-1}}} \\
&\approx{f_t}
\end{aligned} \\
\\
\frac{\partial{c_t}}{\partial{W_f}}=\sum_{i=1}^{t}{\frac{\partial{c_1}}{\partial{W_f}}\prod_{j=1}^{i-1}{f_{j+1}}}
\end{gathered}$$